code/src/internal/internal_definitions.lean
@@ -13,7 +13,7 @@ def Result.is_match : Result → bool
 
 -- Simpler definition of 𝒰 that does not need an accumulator
 def U : Gdt → Φ
-| (Gdt.leaf _) := Φ.false
+| (Gdt.rhs _) := Φ.false
 | (Gdt.branch tr1 tr2) := (U tr1).and (U tr2)
 | (Gdt.grd (Grd.bang var) tree) := ((Φ.var_is_not_bottom var).and (U tree))
 | (Gdt.grd (Grd.xgrd grd) tree) :=
@@ -21,47 +21,47 @@ def U : Gdt → Φ
             .or
                 (Φ.xgrd_in grd (U tree))
 
-def Gdt.mark_all_leaves_inactive: Gdt → Ant bool
-| (Gdt.leaf leaf) := Ant.leaf tt leaf 
-| (Gdt.branch tr1 tr2) := Ant.branch tr1.mark_all_leaves_inactive tr2.mark_all_leaves_inactive
-| (Gdt.grd (Grd.xgrd _) tr) := tr.mark_all_leaves_inactive
-| (Gdt.grd (Grd.bang _) tr) := Ant.diverge tt tr.mark_all_leaves_inactive
+def Gdt.mark_all_rhss_inactive: Gdt → Ant bool
+| (Gdt.rhs rhs) := Ant.rhs tt rhs 
+| (Gdt.branch tr1 tr2) := Ant.branch tr1.mark_all_rhss_inactive tr2.mark_all_rhss_inactive
+| (Gdt.grd (Grd.xgrd _) tr) := tr.mark_all_rhss_inactive
+| (Gdt.grd (Grd.bang _) tr) := Ant.diverge tt tr.mark_all_rhss_inactive
 
-def Gdt.mark_inactive_leaves : Gdt → Env → Ant bool
-| (Gdt.leaf leaf) env := Ant.leaf ff leaf 
+def Gdt.mark_inactive_rhss : Gdt → Env → Ant bool
+| (Gdt.rhs rhs) env := Ant.rhs ff rhs 
 | (Gdt.branch tr1 tr2) env :=
-    Ant.branch (tr1.mark_inactive_leaves env) (
+    Ant.branch (tr1.mark_inactive_rhss env) (
         if (tr1.eval env).is_match then
-            (tr2.mark_all_leaves_inactive)
+            (tr2.mark_all_rhss_inactive)
         else
-            (tr2.mark_inactive_leaves env)
+            (tr2.mark_inactive_rhss env)
     )
 | (Gdt.grd (Grd.xgrd grd) tr) env :=
     match xgrd_eval grd env with
-    | none := tr.mark_all_leaves_inactive
-    | some env' := tr.mark_inactive_leaves env'
+    | none := tr.mark_all_rhss_inactive
+    | some env' := tr.mark_inactive_rhss env'
     end
 | (Gdt.grd (Grd.bang var) tr) env :=
     if is_bottom var env
-    then Ant.diverge ff (tr.mark_all_leaves_inactive)
-    else Ant.diverge tt (tr.mark_inactive_leaves env)
+    then Ant.diverge ff (tr.mark_all_rhss_inactive)
+    else Ant.diverge tt (tr.mark_inactive_rhss env)
 
 -- ######################## Ant ########################
 
-def Ant.leaves_list { α: Type }: Ant α → list Leaf
-| (Ant.leaf a leaf) := [ leaf ]
-| (Ant.branch tr1 tr2) := Ant.leaves_list tr1 ++ Ant.leaves_list tr2
-| (Ant.diverge a tr) := Ant.leaves_list tr
+def Ant.rhss_list { α: Type }: Ant α → list Rhs
+| (Ant.rhs a rhs) := [ rhs ]
+| (Ant.branch tr1 tr2) := Ant.rhss_list tr1 ++ Ant.rhss_list tr2
+| (Ant.diverge a tr) := Ant.rhss_list tr
 
-def Ant.leaves { α: Type } (ant: Ant α): finset Leaf := ant.leaves_list.to_finset
+def Ant.rhss { α: Type } (ant: Ant α): finset Rhs := ant.rhss_list.to_finset
 
-def Ant.disjoint_leaves { α: Type } : Ant α → Prop
-| (Ant.leaf _ leaf) := true
-| (Ant.branch tr1 tr2) := tr1.disjoint_leaves ∧ tr2.disjoint_leaves ∧ disjoint tr1.leaves tr2.leaves
-| (Ant.diverge _ tr) := tr.disjoint_leaves
+def Ant.disjoint_rhss { α: Type } : Ant α → Prop
+| (Ant.rhs _ rhs) := true
+| (Ant.branch tr1 tr2) := tr1.disjoint_rhss ∧ tr2.disjoint_rhss ∧ disjoint tr1.rhss tr2.rhss
+| (Ant.diverge _ tr) := tr.disjoint_rhss
 
 def Ant.map { α β: Type } : (α → β) → Ant α → Ant β
-| f (Ant.leaf a leaf) := Ant.leaf (f a) leaf
+| f (Ant.rhs a rhs) := Ant.rhs (f a) rhs
 | f (Ant.branch tr1 tr2) := (Ant.branch (tr1.map f) (tr2.map f))
 | f (Ant.diverge a tr) := (Ant.diverge (f a) (tr.map f))
 -- TODO: functor implementieren? f <$> ant
@@ -71,18 +71,18 @@ def Ant.map_option { α β: Type } : (α → β) → option (Ant α) → option 
 | f none := none
 -- TODO: fmap?
 
-def Ant.eval_leaves (ant: Ant Φ) (env: Env) := ant.map (λ ty, ty.eval env)
+def Ant.eval_rhss (ant: Ant Φ) (env: Env) := ant.map (λ ty, ty.eval env)
 
-def Ant.mark_inactive_leaves (ant: Ant Φ) (env: Env) := ant.map (λ ty, !(ty.eval env))
+def Ant.mark_inactive_rhss (ant: Ant Φ) (env: Env) := ant.map (λ ty, !(ty.eval env))
 
-def Ant.inactive_leaves : Ant bool → finset Leaf
-| (Ant.leaf inactive n) := if inactive then { n } else ∅
-| (Ant.diverge inactive tr) := tr.inactive_leaves
-| (Ant.branch tr1 tr2) := tr1.inactive_leaves ∪ tr2.inactive_leaves
+def Ant.inactive_rhss : Ant bool → finset Rhs
+| (Ant.rhs inactive n) := if inactive then { n } else ∅
+| (Ant.diverge inactive tr) := tr.inactive_rhss
+| (Ant.branch tr1 tr2) := tr1.inactive_rhss ∪ tr2.inactive_rhss
 
 inductive Ant.implies: Ant bool → Ant bool → Prop
-| leaf { a b: bool } { leaf } (h: a → b):
-    Ant.implies (Ant.leaf a leaf) (Ant.leaf b leaf)
+| rhs { a b: bool } { rhs } (h: a → b):
+    Ant.implies (Ant.rhs a rhs) (Ant.rhs b rhs)
 | branch { a_tr1 a_tr2 b_tr1 b_tr2 } (h1: Ant.implies a_tr1 b_tr1) (h2: Ant.implies a_tr2 b_tr2):
     Ant.implies (Ant.branch a_tr1 a_tr2) (Ant.branch b_tr1 b_tr2)
 | diverge { a b: bool } { a_tr b_tr } (h1: Ant.implies a_tr b_tr) (h2: a → b):
@@ -90,24 +90,24 @@ inductive Ant.implies: Ant bool → Ant bool → Prop
 
 infix `⟶`: 50 := Ant.implies
 
-def Ant.critical_leaf_sets : Ant bool → finset (finset Leaf)
-| (Ant.leaf inactive n) := ∅
-| (Ant.diverge inactive tr) := tr.critical_leaf_sets ∪ if inactive
+def Ant.critical_rhs_sets : Ant bool → finset (finset Rhs)
+| (Ant.rhs inactive n) := ∅
+| (Ant.diverge inactive tr) := tr.critical_rhs_sets ∪ if inactive
     then ∅
-    else { tr.leaves }
-| (Ant.branch tr1 tr2) := tr1.critical_leaf_sets ∪ tr2.critical_leaf_sets
+    else { tr.rhss }
+| (Ant.branch tr1 tr2) := tr1.critical_rhs_sets ∪ tr2.critical_rhs_sets
 
-def Ant.is_redundant_set (a: Ant bool) (leaves: finset Leaf) :=
-    leaves ∩ a.leaves ⊆ a.inactive_leaves
-    ∧ ∀ c ∈ a.critical_leaf_sets, ∃ l ∈ c, l ∉ leaves
+def Ant.is_redundant_set (a: Ant bool) (rhss: finset Rhs) :=
+    rhss ∩ a.rhss ⊆ a.inactive_rhss
+    ∧ ∀ c ∈ a.critical_rhs_sets, ∃ l ∈ c, l ∉ rhss
 -- TODO: rcases
 
--- leaves.redundant_in ant
--- ant.is_redundant_set leaves
+-- rhss.redundant_in ant
+-- ant.is_redundant_set rhss
 
 -- This is a simpler definition of 𝒜 that is semantically equivalent.
 def A : Gdt → Ant Φ
-| (Gdt.leaf leaf) := Ant.leaf Φ.true leaf
+| (Gdt.rhs rhs) := Ant.rhs Φ.true rhs
 | (Gdt.branch tr1 tr2) := Ant.branch (A tr1) $ (A tr2).map ((U tr1).and)
 | (Gdt.grd (Grd.bang var) tr) := Ant.diverge (Φ.var_is_bottom var) $ (A tr).map ((Φ.var_is_not_bottom var).and)
 | (Gdt.grd (Grd.xgrd grd) tr) := (A tr).map (Φ.xgrd_in grd)
@@ -115,22 +115,22 @@ def A : Gdt → Ant Φ
 -- ######################## R ########################
 
 -- (accessible, inaccessible, redundant)
-structure LeafPartition := mk :: (acc : list Leaf) (inacc : list Leaf) (red : list Leaf)
+structure RhsPartition := mk :: (acc : list Rhs) (inacc : list Rhs) (red : list Rhs)
 
-def LeafPartition.leaves (p: LeafPartition) : list Leaf := p.acc ++ p.inacc ++ p.red
+def RhsPartition.rhss (p: RhsPartition) : list Rhs := p.acc ++ p.inacc ++ p.red
 
-def LeafPartition.to_triple (p: LeafPartition): (list Leaf × list Leaf × list Leaf) :=
+def RhsPartition.to_triple (p: RhsPartition): (list Rhs × list Rhs × list Rhs) :=
     (p.acc, p.inacc, p.red)
 
 /-
     This definition is much easier to use than ℛ, but almost equal to ℛ.
     * Associativity of `Ant.map` can be utilized.
-    * LeafPartition is much easier to use than triples.
+    * RhsPartition is much easier to use than triples.
     * Ant.branch has no match which would require a case distinction.
     * This definition can handle any `Ant bool`.
 -/
-def R : Ant bool → LeafPartition
-| (Ant.leaf can_prove_empty n) := if can_prove_empty then ⟨ [], [], [n] ⟩ else ⟨ [n], [], [] ⟩
+def R : Ant bool → RhsPartition
+| (Ant.rhs can_prove_empty n) := if can_prove_empty then ⟨ [], [], [n] ⟩ else ⟨ [n], [], [] ⟩
 | (Ant.diverge can_prove_empty tr) := 
     match R tr, can_prove_empty with
     | ⟨ [], [], m :: ms ⟩, ff := ⟨ [], [m], ms ⟩
