code/src/internal/A.lean
@@ -12,18 +12,18 @@ variable [GuardModule]
 open GuardModule
 
 private lemma A_eq_𝒜' (gdt: Gdt) { acc: Φ → Φ } (acc_stable: stable acc) (acc_hom: hom acc):
-    ((A gdt).map acc).eval_leaves = (𝒜_acc acc gdt).eval_leaves :=
+    ((A gdt).map acc).eval_rhss = (𝒜_acc acc gdt).eval_rhss :=
 begin
     ext env,
     induction gdt generalizing acc env,
-    case Gdt.leaf { simp [A, Ant.map, 𝒜_acc], },
+    case Gdt.rhs { simp [A, Ant.map, 𝒜_acc], },
     case Gdt.branch {
         unfold 𝒜_acc,
-        unfold Ant.eval_leaves,
+        unfold Ant.eval_rhss,
         unfold Ant.map,
-        rw ←Ant.eval_leaves,
-        rw ←Ant.eval_leaves,
-        rw ←Ant.eval_leaves,
+        rw ←Ant.eval_rhss,
+        rw ←Ant.eval_rhss,
+        rw ←Ant.eval_rhss,
         
         specialize gdt_ih_tr1 env acc_stable acc_hom,
         rw ←gdt_ih_tr1,
@@ -33,7 +33,7 @@ begin
             (hom.comp hom.and_right stable.and_right acc_hom acc_stable),
         rw ←gdt_ih_tr2,
 
-        simp [Ant.map, A, Ant.eval_leaves, Ant.map_associative, function.comp, Φ.eval, (acc_hom _ _).2, U_eq_𝒰_acc acc_stable acc_hom],
+        simp [Ant.map, A, Ant.eval_rhss, Ant.map_associative, function.comp, Φ.eval, (acc_hom _ _).2, U_eq_𝒰_acc acc_stable acc_hom],
     },
     case Gdt.grd {
         cases gdt_grd,        
@@ -46,9 +46,9 @@ begin
             rw Ant.map_associative,
         },
         case Grd.bang {
-            unfold A 𝒜_acc Ant.map Ant.eval_leaves,
-            rw ←Ant.eval_leaves,
-            rw ←Ant.eval_leaves,
+            unfold A 𝒜_acc Ant.map Ant.eval_rhss,
+            rw ←Ant.eval_rhss,
+            rw ←Ant.eval_rhss,
             specialize @gdt_ih (acc ∘ (Φ.var_is_not_bottom gdt_grd).and) env
                 (stable.comp acc_stable stable.and_right)
                 (hom.comp acc_hom acc_stable hom.and_right stable.and_right),
@@ -58,7 +58,7 @@ begin
     },
 end
 
-theorem A_eq_𝒜 (gdt: Gdt): (A gdt).eval_leaves = (𝒜 gdt).eval_leaves :=
+theorem A_eq_𝒜 (gdt: Gdt): (A gdt).eval_rhss = (𝒜 gdt).eval_rhss :=
 begin
     unfold 𝒜,
     have := A_eq_𝒜' gdt stable.id hom.id,
@@ -67,36 +67,36 @@ begin
 end
 
 @[simp]
-lemma A_leaves { gdt: Gdt }: (A gdt).leaves = gdt.leaves :=
+lemma A_rhss { gdt: Gdt }: (A gdt).rhss = gdt.rhss :=
 begin
     induction gdt,
-    case Gdt.leaf { finish, },
-    case Gdt.branch { finish [Gdt.leaves, A, Ant.map], },
+    case Gdt.rhs { finish, },
+    case Gdt.branch { finish [Gdt.rhss, A, Ant.map], },
     case Gdt.grd {
         cases gdt_grd;
-        finish [Gdt.leaves, A, Ant.map],
+        finish [Gdt.rhss, A, Ant.map],
     },
 end
 
-lemma Ant.disjoint_leaves_of_gdt_disjoint_leaves { gdt: Gdt } (h: gdt.disjoint_leaves): (A gdt).disjoint_leaves :=
+lemma Ant.disjoint_rhss_of_gdt_disjoint_rhss { gdt: Gdt } (h: gdt.disjoint_rhss): (A gdt).disjoint_rhss :=
 begin
     induction gdt,
-    case Gdt.leaf { simp [A], },
+    case Gdt.rhs { simp [A], },
     case Gdt.branch {
-        unfold Gdt.disjoint_leaves at h,
-        simp [A, Gdt.disjoint_leaves, Ant.disjoint_leaves, *],
+        unfold Gdt.disjoint_rhss at h,
+        simp [A, Gdt.disjoint_rhss, Ant.disjoint_rhss, *],
     },
     case Gdt.grd {
-        unfold Gdt.disjoint_leaves at h,
+        unfold Gdt.disjoint_rhss at h,
         cases gdt_grd;
-        { simp [A, Ant.disjoint_leaves, *], },
+        { simp [A, Ant.disjoint_rhss, *], },
     },
 end
 
-lemma Ant.disjoint_leaves_iff_of_mark_inactive_leaves_eq { ant1 ant2: Ant Φ } { env: Env } (h: ant1.mark_inactive_leaves env = ant2.mark_inactive_leaves env):
-    ant1.disjoint_leaves ↔ ant2.disjoint_leaves :=
+lemma Ant.disjoint_rhss_iff_of_mark_inactive_rhss_eq { ant1 ant2: Ant Φ } { env: Env } (h: ant1.mark_inactive_rhss env = ant2.mark_inactive_rhss env):
+    ant1.disjoint_rhss ↔ ant2.disjoint_rhss :=
 begin
-    have : (ant1.mark_inactive_leaves env).disjoint_leaves ↔ (ant2.mark_inactive_leaves env).disjoint_leaves := by rw h,
+    have : (ant1.mark_inactive_rhss env).disjoint_rhss ↔ (ant2.mark_inactive_rhss env).disjoint_rhss := by rw h,
     simp at this,
     exact this,
 end
