code/src/internal/Ant/map.lean
@@ -20,9 +20,9 @@ lemma Ant.map_id { α: Type } (ant: Ant α): ant.map id = ant :=
 by induction ant; simp [Ant.map, *]
 
 @[simp]
-lemma Ant.map_leaves { α β: Type } (ant: Ant α) (f: α → β): (ant.map f).leaves = ant.leaves :=
-by induction ant; finish [Ant.leaves, Ant.leaves_list, Ant.map]
+lemma Ant.map_rhss { α β: Type } (ant: Ant α) (f: α → β): (ant.map f).rhss = ant.rhss :=
+by induction ant; finish [Ant.rhss, Ant.rhss_list, Ant.map]
 
 @[simp]
-lemma Ant.map_disjoint_leaves_iff { α β: Type } { f: α → β } { ant: Ant α }: (ant.map f).disjoint_leaves ↔ ant.disjoint_leaves :=
-by induction ant; { simp only [Ant.map, Ant.disjoint_leaves, *, Ant.map_leaves], }
+lemma Ant.map_disjoint_rhss_iff { α β: Type } { f: α → β } { ant: Ant α }: (ant.map f).disjoint_rhss ↔ ant.disjoint_rhss :=
+by induction ant; { simp only [Ant.map, Ant.disjoint_rhss, *, Ant.map_rhss], }
