code/src/internal/Gdt/mark_all_rhss_inactive.lean
@@ -1,0 +1,109 @@
+import tactic
+import ...definitions
+import ..internal_definitions
+import ..Ant.main
+import .eval
+
+variable [GuardModule]
+open GuardModule
+
+@[simp]
+lemma Gdt.mark_all_rhss_inactive.inactive_rhss (gdt: Gdt):
+    gdt.mark_all_rhss_inactive.inactive_rhss = gdt.rhss :=
+begin
+    induction gdt;
+    try { cases gdt_grd };
+    simp [*, Gdt.rhss, Gdt.mark_all_rhss_inactive, Ant.inactive_rhss],
+end
+
+@[simp]
+lemma Gdt.mark_all_rhss_inactive.critical_rhs_sets (gdt: Gdt):
+    gdt.mark_all_rhss_inactive.critical_rhs_sets = ∅ :=
+begin
+    induction gdt;
+    try { cases gdt_grd };
+    simp [*, Gdt.rhss, Gdt.mark_all_rhss_inactive, Ant.critical_rhs_sets],
+end
+
+@[simp]
+lemma Gdt.mark_all_rhss_inactive.rhss (gdt: Gdt):
+    gdt.mark_all_rhss_inactive.rhss = gdt.rhss :=
+begin
+    induction gdt;
+    try { cases gdt_grd };
+    simp [*, Gdt.rhss, Gdt.mark_all_rhss_inactive, Ant.critical_rhs_sets],
+end
+
+@[simp]
+lemma Gdt.mark_all_rhss_inactive_map_true (gdt: Gdt):
+    gdt.mark_all_rhss_inactive.map (λ x, tt) = gdt.mark_all_rhss_inactive :=
+begin
+    induction gdt;
+    try { cases gdt_grd };
+    simp [*, Ant.map, Gdt.mark_all_rhss_inactive],
+end
+
+lemma Gdt.mark_all_rhss_inactive_is_reduntant_set (gdt: Gdt) (rhss: finset Rhs): gdt.mark_all_rhss_inactive.is_redundant_set rhss :=
+by simp [Ant.is_redundant_set, finset.inter_subset_right]
+
+
+lemma Gdt.mark_inactive_rhss_of_xgrd_some { xgrd: XGrd } { env env': Env } (h: xgrd_eval xgrd env = some env') (gdt: Gdt):
+    (Gdt.grd (Grd.xgrd xgrd) gdt).mark_inactive_rhss env = gdt.mark_inactive_rhss env' :=
+by simp [Gdt.mark_inactive_rhss, h, Gdt.mark_inactive_rhss._match_1]
+
+lemma Gdt.mark_inactive_rhss_of_xgrd_none { xgrd: XGrd } { env: Env } (h: xgrd_eval xgrd env = none) (gdt: Gdt):
+    (Gdt.grd (Grd.xgrd xgrd) gdt).mark_inactive_rhss env = gdt.mark_all_rhss_inactive :=
+by simp [Gdt.mark_inactive_rhss, h, Gdt.mark_inactive_rhss._match_1]
+
+lemma Gdt.mark_inactive_rhss_map_tt (gdt: Gdt) (env: Env):
+    (gdt.mark_inactive_rhss env).map (λ x, tt) = gdt.mark_all_rhss_inactive :=
+begin
+    induction gdt generalizing env;
+    try { cases gdt_grd };
+    try { cases c: (gdt_tr1.eval env).is_match };
+    try { cases c: (xgrd_eval gdt_grd env) };
+    try { cases c: is_bottom gdt_grd env };
+    simp [*, Gdt.rhss, Gdt.mark_inactive_rhss, Gdt.mark_all_rhss_inactive, Ant.map],
+end
+
+@[simp]
+lemma Gdt.mark_inactive_rhss.rhss (gdt: Gdt) (env: Env):
+    (gdt.mark_inactive_rhss env).rhss = gdt.rhss :=
+begin
+    induction gdt generalizing env;
+    try { cases gdt_grd };
+    try { cases c: (gdt_tr1.eval env).is_match };
+    try { cases c: (xgrd_eval gdt_grd env) };
+    try { cases c: is_bottom gdt_grd env };
+    simp [*, Gdt.rhss, Gdt.mark_inactive_rhss, Ant.critical_rhs_sets],
+end
+
+lemma Gdt.mark_inactive_rhss.inactive_rhss (gdt: Gdt) (env: Env): (gdt.mark_inactive_rhss env).inactive_rhss ⊆ gdt.rhss :=
+by simp only [←Gdt.mark_inactive_rhss.rhss gdt env, Ant.inactive_rhss_subset_rhss]
+
+lemma Gdt.mark_inactive_rhss_no_match { env: Env } { gdt: Gdt } (h: gdt.eval env = Result.no_match):
+    gdt.mark_inactive_rhss env = gdt.mark_all_rhss_inactive :=
+begin
+    induction gdt with rhs generalizing env,
+    case Gdt.rhs { finish [Gdt.eval], },
+    case Gdt.branch {
+        simp [
+            Gdt.mark_inactive_rhss, Gdt.mark_all_rhss_inactive,
+            Gdt.eval_branch_no_match_iff.1 h, *
+        ],
+    },
+    case Gdt.grd {
+        cases gdt_grd with gdt_grd var,
+        case Grd.xgrd {
+            cases c: xgrd_eval gdt_grd env, {
+                simp [Gdt.mark_inactive_rhss, Gdt.mark_all_rhss_inactive, c],
+            }, {
+                rw [Gdt.eval_xgrd_of_some c] at h,
+                simp [Gdt.mark_inactive_rhss, Gdt.mark_all_rhss_inactive, c, gdt_ih h],
+            },
+        },
+        case Grd.bang {
+            simp [Gdt.mark_inactive_rhss, Gdt.mark_all_rhss_inactive, Gdt.eval_bang_no_match_iff.1 h, gdt_ih],
+        },
+    },
+end
