code/src/internal/R.lean
@@ -2,7 +2,7 @@ import tactic
 import data.finset
 import ..definitions
 import .internal_definitions
-import .Ant.leaves
+import .Ant.rhss
 import .utils
 
 variable [GuardModule]
@@ -19,7 +19,7 @@ begin
 end
 
 lemma R_diverge_cases (ant: Ant bool) (a: bool):
-    (∃ rh: Leaf, ∃ rs: list Leaf, a = ff ∧ R ant = ⟨ [], [], rh::rs ⟩ ∧ R (Ant.diverge a ant) = ⟨ [], [rh], rs ⟩)
+    (∃ rh: Rhs, ∃ rs: list Rhs, a = ff ∧ R ant = ⟨ [], [], rh::rs ⟩ ∧ R (Ant.diverge a ant) = ⟨ [], [rh], rs ⟩)
     ∨ ((a = tt ∨ (R ant).acc ≠ [] ∨ (R ant).inacc ≠ [] ∨ (R ant).red = []) ∧ R (Ant.diverge a ant) = R ant) :=
 begin
     unfold R Ant.map,
@@ -32,17 +32,17 @@ begin
     simp [R._match_1],
 end
 
-lemma R_branch_leaves_perm (tr1 tr2: Ant bool) : (R (tr1.branch tr2)).leaves ~ (R tr1).leaves ++ (R tr2).leaves :=
-by simp only [LeafPartition.leaves, R, ←multiset.coe_eq_coe, ←multiset.coe_add, add_left_comm, add_comm]
+lemma R_branch_rhss_perm (tr1 tr2: Ant bool) : (R (tr1.branch tr2)).rhss ~ (R tr1).rhss ++ (R tr2).rhss :=
+by simp only [RhsPartition.rhss, R, ←multiset.coe_eq_coe, ←multiset.coe_add, add_left_comm, add_comm]
 
-lemma R_leaves_perm { ant: Ant bool }:
-    (R ant).leaves ~ ant.leaves_list :=
+lemma R_rhss_perm { ant: Ant bool }:
+    (R ant).rhss ~ ant.rhss_list :=
 begin
     induction ant,
-    case Ant.leaf { cases ant_a; simp [R, LeafPartition.leaves, Ant.leaves_list], },
+    case Ant.rhs { cases ant_a; simp [R, RhsPartition.rhss, Ant.rhss_list], },
     case Ant.branch {
-        unfold Ant.leaves_list,
-        apply list.perm.trans (R_branch_leaves_perm ant_tr1 ant_tr2),
+        unfold Ant.rhss_list,
+        apply list.perm.trans (R_branch_rhss_perm ant_tr1 ant_tr2),
         apply list.perm.append;
         simp *,
     },
@@ -50,38 +50,38 @@ begin
         R_diverge_cases, {
             inline R_ant_tr,
             revert ant_ih,
-            simp [LeafPartition.leaves, Ant.leaves_list],
+            simp [RhsPartition.rhss, Ant.rhss_list],
         }, {
-            simp [Ant.leaves_list, *],
+            simp [Ant.rhss_list, *],
         },
     }
 end
 
-lemma R_leaves_to_finset_eq_leaves { ant: Ant bool }: (R ant).leaves.to_finset = ant.leaves :=
-list_to_finset_eq_of_perm R_leaves_perm
+lemma R_rhss_to_finset_eq_rhss { ant: Ant bool }: (R ant).rhss.to_finset = ant.rhss :=
+list_to_finset_eq_of_perm R_rhss_perm
 
-lemma R_leaves_to_finset_subset_leaves { ant: Ant bool }: (R ant).leaves.to_finset ⊆ ant.leaves :=
-finset.subset_of_eq R_leaves_to_finset_eq_leaves
+lemma R_rhss_to_finset_subset_rhss { ant: Ant bool }: (R ant).rhss.to_finset ⊆ ant.rhss :=
+finset.subset_of_eq R_rhss_to_finset_eq_rhss
 
-lemma R_acc_subset_leaves { ant: Ant bool }: (R ant).acc.to_finset ⊆ ant.leaves :=
-by apply finset.subset.trans _ R_leaves_to_finset_subset_leaves; finish [finset.subset_iff, LeafPartition.leaves]
+lemma R_acc_subset_rhss { ant: Ant bool }: (R ant).acc.to_finset ⊆ ant.rhss :=
+by apply finset.subset.trans _ R_rhss_to_finset_subset_rhss; finish [finset.subset_iff, RhsPartition.rhss]
 
-lemma R_inacc_subset_leaves { ant: Ant bool }: (R ant).inacc.to_finset ⊆ ant.leaves :=
-by apply finset.subset.trans _ R_leaves_to_finset_subset_leaves; finish [finset.subset_iff, LeafPartition.leaves]
+lemma R_inacc_subset_rhss { ant: Ant bool }: (R ant).inacc.to_finset ⊆ ant.rhss :=
+by apply finset.subset.trans _ R_rhss_to_finset_subset_rhss; finish [finset.subset_iff, RhsPartition.rhss]
 
-lemma R_red_subset_leaves { ant: Ant bool }: (R ant).red.to_finset ⊆ ant.leaves :=
-by apply finset.subset.trans _ R_leaves_to_finset_subset_leaves; finish [finset.subset_iff, LeafPartition.leaves]
+lemma R_red_subset_rhss { ant: Ant bool }: (R ant).red.to_finset ⊆ ant.rhss :=
+by apply finset.subset.trans _ R_rhss_to_finset_subset_rhss; finish [finset.subset_iff, RhsPartition.rhss]
 
-lemma R_leaves_nodup { ant: Ant bool } (ant_disjoint: ant.disjoint_leaves): (R ant).leaves.nodup :=
-(list.perm.nodup_iff R_leaves_perm).2 (Ant.leaves_list.nodup ant_disjoint)
+lemma R_rhss_nodup { ant: Ant bool } (ant_disjoint: ant.disjoint_rhss): (R ant).rhss.nodup :=
+(list.perm.nodup_iff R_rhss_perm).2 (Ant.rhss_list.nodup ant_disjoint)
 
-lemma R_red_nodup { ant: Ant bool } (ant_disjoint: ant.disjoint_leaves): (R ant).red.nodup :=
-list.nodup_of_nodup_append_right (R_leaves_nodup ant_disjoint)
+lemma R_red_nodup { ant: Ant bool } (ant_disjoint: ant.disjoint_rhss): (R ant).red.nodup :=
+list.nodup_of_nodup_append_right (R_rhss_nodup ant_disjoint)
 
-lemma R_acc_nodup { ant: Ant bool } (ant_disjoint: ant.disjoint_leaves): (R ant).acc.nodup :=
-list.nodup_of_nodup_append_left (list.nodup_of_nodup_append_left (R_leaves_nodup ant_disjoint))
+lemma R_acc_nodup { ant: Ant bool } (ant_disjoint: ant.disjoint_rhss): (R ant).acc.nodup :=
+list.nodup_of_nodup_append_left (list.nodup_of_nodup_append_left (R_rhss_nodup ant_disjoint))
 
-lemma R_red_l_not_mem_ls { ant: Ant bool } (ant_disjoint: ant.disjoint_leaves) { l: Leaf } { ls: list Leaf } (h: (R ant).red = l::ls):
+lemma R_red_l_not_mem_ls { ant: Ant bool } (ant_disjoint: ant.disjoint_rhss) { l: Rhs } { ls: list Rhs } (h: (R ant).red = l::ls):
     l ∉ ls.to_finset :=
 begin
     have := R_red_nodup ant_disjoint,
@@ -89,22 +89,22 @@ begin
     simp [list.not_mem_of_nodup_cons this],
 end
 
-lemma R_acc_l_not_mem_red { ant: Ant bool } (ant_disjoint: ant.disjoint_leaves) { l: Leaf } { ls: list Leaf } (h: (R ant).acc = l::ls):
+lemma R_acc_l_not_mem_red { ant: Ant bool } (ant_disjoint: ant.disjoint_rhss) { l: Rhs } { ls: list Rhs } (h: (R ant).acc = l::ls):
     l ∉ (R ant).red.to_finset :=
 begin
-    have := R_leaves_nodup ant_disjoint,
-    unfold LeafPartition.leaves at this,
+    have := R_rhss_nodup ant_disjoint,
+    unfold RhsPartition.rhss at this,
     have d := list.disjoint_of_nodup_append this,
     have : l ∈ ((R ant).acc ++ (R ant).inacc) := by simp [h],
     suffices : l ∉ (R ant).red, { simp [this], },
     exact imp_false.mp (@d l this),
 end
 
-lemma R_inacc_l_not_mem_red { ant: Ant bool } (ant_disjoint: ant.disjoint_leaves) { l: Leaf } { ls: list Leaf } (h: (R ant).inacc = l::ls):
+lemma R_inacc_l_not_mem_red { ant: Ant bool } (ant_disjoint: ant.disjoint_rhss) { l: Rhs } { ls: list Rhs } (h: (R ant).inacc = l::ls):
     l ∉ (R ant).red.to_finset :=
 begin
-    have := R_leaves_nodup ant_disjoint,
-    unfold LeafPartition.leaves at this,
+    have := R_rhss_nodup ant_disjoint,
+    unfold RhsPartition.rhss at this,
     have d := list.disjoint_of_nodup_append this,
     have : l ∈ ((R ant).acc ++ (R ant).inacc) := by simp [h],
     suffices : l ∉ (R ant).red, { simp [this], },
@@ -114,9 +114,9 @@ end
 lemma R_eq_ℛ (can_prove_empty: Φ → bool) (ant: Ant Φ): (R (ant.map can_prove_empty)).to_triple = ℛ can_prove_empty ant :=
 begin
     induction ant,
-    case Ant.leaf {
+    case Ant.rhs {
         cases c: can_prove_empty ant_a;
-        simp [R, R._match_1, ℛ, ℛ._match_1, Ant.map, ℛ._match_2, LeafPartition.to_triple, c],
+        simp [R, R._match_1, ℛ, ℛ._match_1, Ant.map, ℛ._match_2, RhsPartition.to_triple, c],
     },
     case Ant.branch {
         rw ℛ,
@@ -126,7 +126,7 @@ begin
         cases ir1 with i1 r1;
         cases ℛ can_prove_empty ant_tr2 with a2 ir2;
         cases ir2 with i2 r2;
-        simp [R, R._match_1, ℛ, ℛ._match_1, Ant.map, ℛ._match_2, LeafPartition.to_triple],
+        simp [R, R._match_1, ℛ, ℛ._match_1, Ant.map, ℛ._match_2, RhsPartition.to_triple],
     },
     case Ant.diverge {
         rw ℛ,
@@ -136,6 +136,6 @@ begin
         cases acc;
         cases inacc;
         cases red;
-        simp [R, R._match_1, ℛ, ℛ._match_1, Ant.map, ℛ._match_2, LeafPartition.to_triple, c1, c],
+        simp [R, R._match_1, ℛ, ℛ._match_1, Ant.map, ℛ._match_2, RhsPartition.to_triple, c1, c],
     },
 end
