code/src/internal/R_red_removable.lean
@@ -14,34 +14,34 @@ import .R
 variable [GuardModule]
 open GuardModule
 
-lemma R_red_redundant { ant: Ant bool } (ant_disjoint: ant.disjoint_leaves):
+lemma R_red_redundant { ant: Ant bool } (ant_disjoint: ant.disjoint_rhss):
     ant.is_redundant_set (R ant).red.to_finset :=
 begin
     induction_ant_disjoint ant from ant_disjoint,
 
-    case Ant.leaf {
+    case Ant.rhs {
         unfold Ant.is_redundant_set R,
         cases ant_a;
-        simp [Ant.critical_leaf_sets, Ant.inactive_leaves],
+        simp [Ant.critical_rhs_sets, Ant.inactive_rhss],
     },
     case Ant.branch {
         unfold Ant.is_redundant_set R,
         unfold Ant.is_redundant_set R at ant_ih_tr1,
         unfold Ant.is_redundant_set R at ant_ih_tr2,
-        unfold LeafPartition.red,
+        unfold RhsPartition.red,
         split, {
-            simp [Ant.inactive_leaves, finset.union_subset_union ant_ih_tr1.1 ant_ih_tr2.1],
+            simp [Ant.inactive_rhss, finset.union_subset_union ant_ih_tr1.1 ant_ih_tr2.1],
             replace ant_ih_tr1 := ant_ih_tr1.1,
             replace ant_ih_tr2 := ant_ih_tr2.1,
-            rw subset_inter_subset_subset R_red_subset_leaves at ant_ih_tr1,
-            rw subset_inter_subset_subset R_red_subset_leaves at ant_ih_tr2,
+            rw subset_inter_subset_subset R_red_subset_rhss at ant_ih_tr1,
+            rw subset_inter_subset_subset R_red_subset_rhss at ant_ih_tr2,
             apply subset_inter_subset,
             exact finset.union_subset_union ant_ih_tr1 ant_ih_tr2,
         },
 
         assume e,
         assume h,
-        rw Ant.critical_leaf_sets at h,
+        rw Ant.critical_rhs_sets at h,
         
         replace ant_ih_tr1 := ant_ih_tr1.2,
         replace ant_ih_tr2 := ant_ih_tr2.2,
@@ -54,8 +54,8 @@ begin
             have : x ∉ (R ant_tr2).red.to_finset :=
             begin
                 by_contradiction,
-                have h1 := finset.subset_iff.1 (Ant.critical_leaf_set_elements h) H,
-                have h2 := finset.subset_iff.1 (R_red_subset_leaves) a,
+                have h1 := finset.subset_iff.1 (Ant.critical_rhs_set_elements h) H,
+                have h2 := finset.subset_iff.1 (R_red_subset_rhss) a,
                 have := finset.disjoint_iff_ne.1 ant_disjoint _ h1 _ h2,
                 simp at this,
                 exact this,
@@ -71,8 +71,8 @@ begin
             have : x ∉ (R ant_tr1).red.to_finset :=
             begin
                 by_contradiction,
-                have h1 := finset.subset_iff.1 (Ant.critical_leaf_set_elements h) H,
-                have h2 := finset.subset_iff.1 (R_red_subset_leaves) a,
+                have h1 := finset.subset_iff.1 (Ant.critical_rhs_set_elements h) H,
+                have h2 := finset.subset_iff.1 (R_red_subset_rhss) a,
                 have := finset.disjoint_iff_ne.1 ant_disjoint _ h2 _ h1,
                 simp at this,
                 exact this,
@@ -88,8 +88,8 @@ begin
             R_diverge_cases,
             {
                 inline R_ant_tr,
-                unfold LeafPartition.red at *,
-                simp only [Ant.inactive_leaves, Ant.leaves_diverge],
+                unfold RhsPartition.red at *,
+                simp only [Ant.inactive_rhss, Ant.rhss_diverge],
                 have : rs.to_finset ⊆ (r :: rs).to_finset := by simp [finset.subset_insert],
                 have := finset.inter_subset_inter this (finset.subset.refl _),
                 exact finset.subset.trans this ant_ih.1,
@@ -102,13 +102,13 @@ begin
         assume e,
         assume h,
 
-        unfold Ant.critical_leaf_sets at h,
+        unfold Ant.critical_rhs_sets at h,
 
         R_diverge_cases, {
             inline ant_a,
             simp only [bool.coe_sort_ff, if_false, finset.mem_union, finset.mem_singleton] at h,
             rw R_ant_tr at *,
-            unfold LeafPartition.red at *,
+            unfold RhsPartition.red at *,
             cases h, {
                 have := ant_ih.2 e h,
                 cases this with x this,
@@ -119,7 +119,7 @@ begin
                 use r,
                 rw h,
                 have : r ∈ (R ant_tr).red.to_finset := by simp *,
-                have := finset.subset_iff.1 R_red_subset_leaves this,
+                have := finset.subset_iff.1 R_red_subset_rhss this,
                 split, { exact this, },
                 apply R_red_l_not_mem_ls ant_disjoint,
                 simp *,
@@ -143,16 +143,16 @@ begin
                 cases c: (R ant_tr).acc with acc accs, { finish, },
                 use acc,
                 have acc_mem : acc ∈ (R ant_tr).acc.to_finset := by simp [c],
-                simp [finset.subset_iff.1 R_acc_subset_leaves acc_mem, R_acc_l_not_mem_red ant_disjoint c],
+                simp [finset.subset_iff.1 R_acc_subset_rhss acc_mem, R_acc_l_not_mem_red ant_disjoint c],
             },
             cases R_diverge_cases, {
                 cases c: (R ant_tr).inacc with inacc inaccs, { finish, },
                 use inacc,
                 have inacc_mem : inacc ∈ (R ant_tr).inacc.to_finset := by simp [c],
-                simp [finset.subset_iff.1 R_inacc_subset_leaves inacc_mem, R_inacc_l_not_mem_red ant_disjoint c],
+                simp [finset.subset_iff.1 R_inacc_subset_rhss inacc_mem, R_inacc_l_not_mem_red ant_disjoint c],
             },
             {
-                have := Ant.leaves_non_empty ant_tr,
+                have := Ant.rhss_non_empty ant_tr,
                 cases this with l ls,
                 rw R_diverge_cases,
                 use l,
@@ -163,7 +163,7 @@ begin
 end
 
 lemma can_prove_empty_implies_inactive (can_prove_empty: Gs) (ant: Ant Φ) (env: Env):
-    (ant.map (can_prove_empty.val)) ⟶ (ant.mark_inactive_leaves env) :=
+    (ant.map (can_prove_empty.val)) ⟶ (ant.mark_inactive_rhss env) :=
 begin
     have : ∀ ty: Φ, (can_prove_empty.val ty) → !ty.eval env := begin
         unfold_coes,
@@ -174,35 +174,35 @@ begin
     end,
 
     induction ant,
-    case Ant.leaf {
-        apply Ant.implies.leaf,
+    case Ant.rhs {
+        apply Ant.implies.rhs,
         exact this _,
     },
     case Ant.branch {
-        simp only [Ant.implies.branch, Ant.map, Ant.mark_inactive_leaves.branch, *],
+        simp only [Ant.implies.branch, Ant.map, Ant.mark_inactive_rhss.branch, *],
     },
     case Ant.diverge {
-        rw Ant.mark_inactive_leaves_of_diverge,
+        rw Ant.mark_inactive_rhss_of_diverge,
         apply Ant.implies.diverge ant_ih (this _),
     },
 end
 
-lemma A_mark_inactive_leaves (gdt: Gdt) (env: Env): (A gdt).mark_inactive_leaves env = gdt.mark_inactive_leaves env :=
+lemma A_mark_inactive_rhss (gdt: Gdt) (env: Env): (A gdt).mark_inactive_rhss env = gdt.mark_inactive_rhss env :=
 begin
     have : bor ff = id := by refl,
     have : bor tt = λ x, tt := by refl,
     induction gdt generalizing env,
-    case Gdt.leaf { refl, },
+    case Gdt.rhs { refl, },
     case Gdt.branch {
         unfold A,
-        rw Ant.mark_inactive_leaves_branch,
-        rw Ant.mark_inactive_leaves_of_map_ty_and _ _ _,
+        rw Ant.mark_inactive_rhss_branch,
+        rw Ant.mark_inactive_rhss_of_map_ty_and _ _ _,
         rw [gdt_ih_tr1, gdt_ih_tr2],
         rw U_semantic,
-        unfold Gdt.mark_inactive_leaves,
+        unfold Gdt.mark_inactive_rhss,
         simp only [true_and, eq_self_iff_true, ne.def, bnot_bnot],
         cases (gdt_tr1.eval env).is_match;
-        simp [*, Gdt.mark_inactive_leaves_map_tt],
+        simp [*, Gdt.mark_inactive_rhss_map_tt],
     },
     case Gdt.grd {
         cases gdt_grd,
@@ -210,55 +210,55 @@ begin
             unfold A,
             cases c: xgrd_eval gdt_grd env,
             case option.none {
-                rw [Ant.mark_inactive_leaves_of_map_xgrd_in_none c, Gdt.mark_inactive_leaves_of_xgrd_none c],
-                rw ←Gdt.mark_inactive_leaves_map_tt _ env,
+                rw [Ant.mark_inactive_rhss_of_map_xgrd_in_none c, Gdt.mark_inactive_rhss_of_xgrd_none c],
+                rw ←Gdt.mark_inactive_rhss_map_tt _ env,
                 rw ←gdt_ih env,
-                simp [Ant.mark_inactive_leaves],
+                simp [Ant.mark_inactive_rhss],
             },
             case option.some {
-                rw Ant.mark_inactive_leaves_of_map_xgrd_in_some c,
-                rw Gdt.mark_inactive_leaves_of_xgrd_some c,
+                rw Ant.mark_inactive_rhss_of_map_xgrd_in_some c,
+                rw Gdt.mark_inactive_rhss_of_xgrd_some c,
                 exact gdt_ih val,
             },
         },
         case Grd.bang {
             unfold A,
-            rw Ant.mark_inactive_leaves_of_diverge,
-            rw Ant.mark_inactive_leaves_of_map_ty_and,
+            rw Ant.mark_inactive_rhss_of_diverge,
+            rw Ant.mark_inactive_rhss_of_map_ty_and,
             rw gdt_ih env,
-            unfold Gdt.mark_inactive_leaves,
+            unfold Gdt.mark_inactive_rhss,
             cases c: is_bottom gdt_grd env;
-            simp [c, *, Gdt.mark_inactive_leaves_map_tt],
+            simp [c, *, Gdt.mark_inactive_rhss_map_tt],
         },
     },
 end
 
 
 lemma is_redundant_set_monotonous' { a b: Ant bool } (h: a ⟶ b): 
-        a.inactive_leaves ⊆ b.inactive_leaves ∧ b.critical_leaf_sets ⊆ a.critical_leaf_sets :=
+        a.inactive_rhss ⊆ b.inactive_rhss ∧ b.critical_rhs_sets ⊆ a.critical_rhs_sets :=
 begin
     induction a generalizing b;
     cases h with h b_a,
-    -- case leaf:
+    -- case rhs:
     {
         cases a_a; cases b_a;
-        finish [Ant.inactive_leaves, Ant.implies.leaf],
+        finish [Ant.inactive_rhss, Ant.implies.rhs],
     },
     -- case branch:
     {
         specialize a_ih_tr1 h_h1,
         specialize a_ih_tr2 h_h2,
-        simp [ *, finset.union_subset_union, Ant.inactive_leaves, Ant.critical_leaf_sets ],
+        simp [ *, finset.union_subset_union, Ant.inactive_rhss, Ant.critical_rhs_sets ],
     },
     -- case grd:
     {
         specialize a_ih h_h1,
-        split, { simp [Ant.inactive_leaves, a_ih], },
+        split, { simp [Ant.inactive_rhss, a_ih], },
 
         cases a_a; cases h_b;
         finish [
-            Ant.critical_leaf_sets,
-            Ant.implies_same_leaves h_h1,
+            Ant.critical_rhs_sets,
+            Ant.implies_same_rhss h_h1,
             finset.union_subset_union,
             a_ih.2,
             subset_right_union
@@ -266,15 +266,15 @@ begin
     },
 end
 
-lemma is_redundant_set_monotonous { a b: Ant bool } (leaves: finset Leaf) (h: a ⟶ b):
-    a.is_redundant_set leaves → b.is_redundant_set leaves :=
+lemma is_redundant_set_monotonous { a b: Ant bool } (rhss: finset Rhs) (h: a ⟶ b):
+    a.is_redundant_set rhss → b.is_redundant_set rhss :=
 begin
     unfold Ant.is_redundant_set,
     have := is_redundant_set_monotonous' h,
     assume p,
     split,
     {
-        rw ←Ant.implies_same_leaves h,
+        rw ←Ant.implies_same_rhss h,
         exact finset.subset.trans p.1 this.1,
     },
     assume e,
@@ -321,50 +321,50 @@ begin
     tauto, 
 end
 
-lemma redundant_leaves_removable
-    (gdt: Gdt) (gdt_disjoint: gdt.disjoint_leaves)
+lemma redundant_rhss_removable
+    (gdt: Gdt) (gdt_disjoint: gdt.disjoint_rhss)
     (env: Env)
-    (leaves: finset Leaf) (leaves_def: (gdt.mark_inactive_leaves env).is_redundant_set leaves):
+    (rhss: finset Rhs) (rhss_def: (gdt.mark_inactive_rhss env).is_redundant_set rhss):
 
-        Gdt.eval_option (gdt.remove_leaves leaves) env = gdt.eval env :=
+        Gdt.eval_option (gdt.remove_rhss rhss) env = gdt.eval env :=
 begin
-  induction gdt with leaf generalizing env,
-  case Gdt.leaf {
+  induction gdt with rhs generalizing env,
+  case Gdt.rhs {
       simp [Gdt.eval],
-      unfold Gdt.mark_inactive_leaves Ant.is_redundant_set at leaves_def,
-      simp [Ant.inactive_leaves, Ant.critical_leaf_sets, Ant.leaves] at leaves_def,
-      unfold Gdt.remove_leaves,
-      have : ¬leaf ∈ leaves := finset.disjoint_singleton.mp leaves_def,
+      unfold Gdt.mark_inactive_rhss Ant.is_redundant_set at rhss_def,
+      simp [Ant.inactive_rhss, Ant.critical_rhs_sets, Ant.rhss] at rhss_def,
+      unfold Gdt.remove_rhss,
+      have : ¬rhs ∈ rhss := finset.disjoint_singleton.mp rhss_def,
       simp [this, Gdt.eval_option],
   },
 
   case Gdt.branch {
-        simp [Gdt.mark_inactive_leaves, -Result.is_match_neq_no_match] at leaves_def,
-        unfold Gdt.remove_leaves,
-        unfold Gdt.disjoint_leaves at gdt_disjoint,
+        simp [Gdt.mark_inactive_rhss, -Result.is_match_neq_no_match] at rhss_def,
+        unfold Gdt.remove_rhss,
+        unfold Gdt.disjoint_rhss at gdt_disjoint,
 
         cases c: (gdt_tr1.eval env).is_match,
         
         case bool.ff {
-            rw c at leaves_def,
+            rw c at rhss_def,
             simp at c,
-            simp only [Ant.inactive_leaves, Ant.is_redundant_set, Ant.critical_leaf_sets, bool.coe_sort_ff, Gdt.mark_inactive_leaves.leaves,
-                Ant.leaves_branch, if_false, finset.mem_union, Gdt.mark_inactive_leaves_no_match c, finset.not_mem_empty, false_or,
-                Gdt.mark_all_leaves_inactive.critical_leaf_sets, Gdt.mark_all_leaves_inactive.inactive_leaves,
-                Gdt.mark_all_leaves_inactive.leaves] at leaves_def,
+            simp only [Ant.inactive_rhss, Ant.is_redundant_set, Ant.critical_rhs_sets, bool.coe_sort_ff, Gdt.mark_inactive_rhss.rhss,
+                Ant.rhss_branch, if_false, finset.mem_union, Gdt.mark_inactive_rhss_no_match c, finset.not_mem_empty, false_or,
+                Gdt.mark_all_rhss_inactive.critical_rhs_sets, Gdt.mark_all_rhss_inactive.inactive_rhss,
+                Gdt.mark_all_rhss_inactive.rhss] at rhss_def,
                             
 
-            have : (gdt_tr1.mark_inactive_leaves env).is_redundant_set leaves :=
-            by simp [Gdt.mark_inactive_leaves_no_match c, Gdt.mark_all_leaves_inactive_is_reduntant_set],
+            have : (gdt_tr1.mark_inactive_rhss env).is_redundant_set rhss :=
+            by simp [Gdt.mark_inactive_rhss_no_match c, Gdt.mark_all_rhss_inactive_is_reduntant_set],
 
             specialize gdt_ih_tr1 gdt_disjoint.1 env this,
 
-            have : (gdt_tr2.mark_inactive_leaves env).is_redundant_set leaves :=
+            have : (gdt_tr2.mark_inactive_rhss env).is_redundant_set rhss :=
             begin
-                have := sets_1 leaves_def.1 gdt_disjoint.2.2,
+                have := sets_1 rhss_def.1 gdt_disjoint.2.2,
                 unfold Ant.is_redundant_set,
                 split, { simp [*], },
-                exact leaves_def.2,
+                exact rhss_def.2,
             end,
 
             specialize gdt_ih_tr2 gdt_disjoint.2.1 env this,
@@ -375,19 +375,19 @@ begin
             simp,
         },
         case bool.tt {
-            rw c at leaves_def,
+            rw c at rhss_def,
             simp only [Result.is_match_tt_neq_no_match, ne.def] at c,
-            simp only [Ant.inactive_leaves, Ant.is_redundant_set, Ant.critical_leaf_sets, exists_prop, Gdt.mark_all_leaves_inactive.leaves,
-                if_true, bool.coe_sort_tt, Gdt.mark_inactive_leaves.leaves, Ant.leaves_branch, finset.union_empty,
-                Gdt.mark_all_leaves_inactive.critical_leaf_sets, Gdt.mark_all_leaves_inactive.inactive_leaves] at leaves_def,
+            simp only [Ant.inactive_rhss, Ant.is_redundant_set, Ant.critical_rhs_sets, exists_prop, Gdt.mark_all_rhss_inactive.rhss,
+                if_true, bool.coe_sort_tt, Gdt.mark_inactive_rhss.rhss, Ant.rhss_branch, finset.union_empty,
+                Gdt.mark_all_rhss_inactive.critical_rhs_sets, Gdt.mark_all_rhss_inactive.inactive_rhss] at rhss_def,
             
-            have : (gdt_tr1.mark_inactive_leaves env).is_redundant_set leaves :=
+            have : (gdt_tr1.mark_inactive_rhss env).is_redundant_set rhss :=
             begin
                 unfold Ant.is_redundant_set,
                 simp,
-                have := sets_2 leaves_def.1 gdt_disjoint.2.2,
+                have := sets_2 rhss_def.1 gdt_disjoint.2.2,
                 split, { simp [*], },
-                exact leaves_def.2,
+                exact rhss_def.2,
             end,
             specialize gdt_ih_tr1 gdt_disjoint.1 env this,
             rw ←Gdt.eval_option at c,
@@ -400,28 +400,28 @@ begin
     },
 
     case Gdt.grd {
-        unfold Gdt.disjoint_leaves at gdt_disjoint,
+        unfold Gdt.disjoint_rhss at gdt_disjoint,
         cases gdt_grd with gdt_grd var,
         case Grd.xgrd {
             cases c: xgrd_eval gdt_grd env with env',
             case option.some {
                 simp only [Gdt.eval_xgrd_of_some c],
-                unfold Ant.is_redundant_set at leaves_def,
-                simp only [Gdt.mark_inactive_leaves, Gdt.mark_inactive_leaves._match_1, c] at leaves_def,
-                have : (gdt_tr.mark_inactive_leaves env').is_redundant_set leaves :=
+                unfold Ant.is_redundant_set at rhss_def,
+                simp only [Gdt.mark_inactive_rhss, Gdt.mark_inactive_rhss._match_1, c] at rhss_def,
+                have : (gdt_tr.mark_inactive_rhss env').is_redundant_set rhss :=
                 begin
                     unfold Ant.is_redundant_set,
-                    exact leaves_def,
+                    exact rhss_def,
                 end,
                 
                 specialize gdt_ih gdt_disjoint env' this,
-                unfold Gdt.remove_leaves,
+                unfold Gdt.remove_rhss,
                 rw Gdt.eval_option_of_xgrd_eval_some c,
                 exact gdt_ih,
             },
             case option.none {
                 simp only [Gdt.eval_xgrd_of_none c],
-                unfold Gdt.remove_leaves,
+                unfold Gdt.remove_rhss,
                 exact Gdt.eval_option_of_xgrd_eval_none c,
             },
         },
@@ -429,21 +429,21 @@ begin
             cases c: is_bottom var env,
             case bool.tt {
                 simp [Gdt.eval_bang_of_bottom c],
-                simp only [Ant.is_redundant_set, Ant.inactive_leaves, Ant.critical_leaf_sets, Gdt.mark_inactive_leaves, c,
-                    Gdt.mark_all_leaves_inactive.leaves, if_true, Ant.leaves_diverge, finset.empty_union, bool.coe_sort_ff,
-                    bool.coe_sort_tt, forall_eq, Gdt.mark_all_leaves_inactive.critical_leaf_sets, if_false, finset.mem_singleton,
-                    Gdt.mark_all_leaves_inactive.inactive_leaves] at leaves_def,
-                unfold Gdt.remove_leaves,
-                apply Gdt.eval_option_of_is_bottom_tt c (Gdt.remove_leaves_neq_none leaves_def.2),
+                simp only [Ant.is_redundant_set, Ant.inactive_rhss, Ant.critical_rhs_sets, Gdt.mark_inactive_rhss, c,
+                    Gdt.mark_all_rhss_inactive.rhss, if_true, Ant.rhss_diverge, finset.empty_union, bool.coe_sort_ff,
+                    bool.coe_sort_tt, forall_eq, Gdt.mark_all_rhss_inactive.critical_rhs_sets, if_false, finset.mem_singleton,
+                    Gdt.mark_all_rhss_inactive.inactive_rhss] at rhss_def,
+                unfold Gdt.remove_rhss,
+                apply Gdt.eval_option_of_is_bottom_tt c (Gdt.remove_rhss_neq_none rhss_def.2),
             },
             case bool.ff {
-                simp [Ant.is_redundant_set, Gdt.leaves, Gdt.mark_inactive_leaves, c, Ant.inactive_leaves, Ant.critical_leaf_sets] at leaves_def,
-                have : (gdt_tr.mark_inactive_leaves env).is_redundant_set leaves, {
-                    simp [Ant.is_redundant_set, Gdt.leaves, Gdt.mark_inactive_leaves, c, Ant.inactive_leaves, Ant.critical_leaf_sets],
-                    exact leaves_def,
+                simp [Ant.is_redundant_set, Gdt.rhss, Gdt.mark_inactive_rhss, c, Ant.inactive_rhss, Ant.critical_rhs_sets] at rhss_def,
+                have : (gdt_tr.mark_inactive_rhss env).is_redundant_set rhss, {
+                    simp [Ant.is_redundant_set, Gdt.rhss, Gdt.mark_inactive_rhss, c, Ant.inactive_rhss, Ant.critical_rhs_sets],
+                    exact rhss_def,
                 },
                 specialize gdt_ih gdt_disjoint env this,
-                unfold Gdt.remove_leaves,
+                unfold Gdt.remove_rhss,
                 simp [Gdt.eval_bang_of_not_bottom c],
                 rw Gdt.eval_option_of_is_bottom_ff c,
                 exact gdt_ih,
@@ -454,10 +454,10 @@ end
 
 theorem R_red_removable
     (can_prove_empty: Gs)
-    { gdt: Gdt } (gdt_disjoint: gdt.disjoint_leaves)
+    { gdt: Gdt } (gdt_disjoint: gdt.disjoint_rhss)
     { Agdt: Ant Φ }
-    (ant_def: Agdt.mark_inactive_leaves = (A gdt).mark_inactive_leaves):
-    Gdt.eval_option (gdt.remove_leaves ((R $ Agdt.map can_prove_empty.val).red.to_finset)) = gdt.eval :=
+    (ant_def: Agdt.mark_inactive_rhss = (A gdt).mark_inactive_rhss):
+    Gdt.eval_option (gdt.remove_rhss ((R $ Agdt.map can_prove_empty.val).red.to_finset)) = gdt.eval :=
 begin
     ext env:1,
     
@@ -467,31 +467,31 @@ begin
 
     -- `can_prove_empty` approximates emptiness for a single refinement type.
     -- `ant_empt` approximates emptiness of the refinement types in `Agdt` for every `env`.
-    -- It also approximates inactive leaves of `gdt` in context of `env` (ant_empt_imp_gdt).
+    -- It also approximates inactive rhss of `gdt` in context of `env` (ant_empt_imp_gdt).
     let ant_empt := Agdt.map can_prove_empty.val,
     have ant_empt_imp_gdt := calc
-        ant_empt ⟶ Agdt.mark_inactive_leaves env : can_prove_empty_implies_inactive can_prove_empty Agdt env
-        ...      ⟶ (A gdt).mark_inactive_leaves env : by simp [Ant.implies_refl, ant_def]
-        ...      ⟶ gdt.mark_inactive_leaves env : by simp [Ant.implies_refl, A_mark_inactive_leaves gdt env],
+        ant_empt ⟶ Agdt.mark_inactive_rhss env : can_prove_empty_implies_inactive can_prove_empty Agdt env
+        ...      ⟶ (A gdt).mark_inactive_rhss env : by simp [Ant.implies_refl, ant_def]
+        ...      ⟶ gdt.mark_inactive_rhss env : by simp [Ant.implies_refl, A_mark_inactive_rhss gdt env],
 
-    -- Since `gdt` has disjoint leaves, `ant_empt` has disjoint leaves too.
-    have ant_empt_disjoint : ant_empt.disjoint_leaves
-        := by simp [Ant.disjoint_leaves_of_gdt_disjoint_leaves gdt_disjoint,
-                Ant.disjoint_leaves_iff_of_mark_inactive_leaves_eq (function.funext_iff.1 ant_def env)],
+    -- Since `gdt` has disjoint rhss, `ant_empt` has disjoint rhss too.
+    have ant_empt_disjoint : ant_empt.disjoint_rhss
+        := by simp [Ant.disjoint_rhss_of_gdt_disjoint_rhss gdt_disjoint,
+                Ant.disjoint_rhss_iff_of_mark_inactive_rhss_eq (function.funext_iff.1 ant_def env)],
 
-    -- The set of leaves `R_red` is redundant in `ant_empt` (red_in_ant_empt).
-    -- This means that these leaves are inactive
-    -- and not all leaves of possibly active diverge nodes are redundant.
+    -- The set of rhss `R_red` is redundant in `ant_empt` (red_in_ant_empt).
+    -- This means that these rhss are inactive
+    -- and not all rhss of possibly active diverge nodes are redundant.
     let R_red := (R ant_empt).red.to_finset,
     have red_in_ant_empt: ant_empt.is_redundant_set R_red := R_red_redundant ant_empt_disjoint,
     
-    -- Since `redundant_in` is monotonous and `ant_empt` approximates inactive leaves on `gdt`,
+    -- Since `redundant_in` is monotonous and `ant_empt` approximates inactive rhss on `gdt`,
     -- `R_red` is also redundant in `gdt` (red_in_gdt).
-    have red_in_gdt: (gdt.mark_inactive_leaves env).is_redundant_set R_red
+    have red_in_gdt: (gdt.mark_inactive_rhss env).is_redundant_set R_red
         := is_redundant_set_monotonous _ ant_empt_imp_gdt red_in_ant_empt,
     
     -- Since `R_red` is a redundant set, it can be removed from `gdt` without
     -- changing the semantics. Note that `R_red` is independent of env.
-    show Gdt.eval_option (Gdt.remove_leaves R_red gdt) env = gdt.eval env,
-    from redundant_leaves_removable gdt gdt_disjoint env _ red_in_gdt,
+    show Gdt.eval_option (Gdt.remove_rhss R_red gdt) env = gdt.eval env,
+    from redundant_rhss_removable gdt gdt_disjoint env _ red_in_gdt,
 end
